Define Chase Trees and start porting results

ProofLibrary/ChaseSequence.lean
@@ -1,181 +1,350 @@
 import ProofLibrary.KnowledgeBaseBasics
 import ProofLibrary.Trigger
 import ProofLibrary.Logic
+import ProofLibrary.PossiblyInfiniteTree
 
-def InfiniteList (α : Type u) := Nat → α  
+def exists_trigger_opt_fs (obs : ObsoletenessCondition) (rules : RuleSet) (before : FactSet) (after : Option FactSet) : Prop :=
+  ∃ trg : (RTrigger obs rules), trg.val.active before ∧ ∃ i, some (before ∪ trg.val.result.get i) = after
 
-structure ChaseSequence (obs : ObsoletenessCondition) (kb : KnowledgeBase) where
-  fact_sets : InfiniteList FactSet
-  database_first : fact_sets 0 = kb.db
-  triggers_exist : ∀ n : Nat, (
-      ∃ trg : (RTrigger obs kb.rules), trg.val.active (fact_sets n) ∧ trg.val.result ∪ fact_sets n = fact_sets (n + 1)
-    ) ∨ (
-      ¬(∃ trg : (RTrigger obs kb.rules), trg.val.active (fact_sets n)) ∧ fact_sets n = fact_sets (n + 1)
-    )
-  fairness : ∀ (trg : (RTrigger obs kb.rules)) (i : Nat), (trg.val.active (fact_sets i)) → ∃ j : Nat, j ≥ i ∧ (¬ trg.val.active (fact_sets j))
+def exists_trigger_list (obs : ObsoletenessCondition) (rules : RuleSet) (before : FactSet) (after : List FactSet) : Prop :=
+  ∃ trg : (RTrigger obs rules), trg.val.active before ∧ trg.val.result.map (fun fs => before ∪ fs) = after
 
-namespace ChaseSequence
-  def result (cs : ChaseSequence obs kb) : FactSet := fun f => ∃ n : Nat, f ∈ cs.fact_sets n
+def not_exists_trigger_opt_fs (obs : ObsoletenessCondition) (rules : RuleSet) (before : FactSet) (after : Option FactSet) : Prop :=
+  ¬(∃ trg : (RTrigger obs rules), trg.val.active before) ∧ after = none
 
-  def terminates (cs : ChaseSequence obs kb) : Prop :=
-    ∃ n : Nat, cs.fact_sets n = cs.fact_sets (n + 1)
-end ChaseSequence
+def not_exists_trigger_list (obs : ObsoletenessCondition) (rules : RuleSet) (before : FactSet) (after : List FactSet) : Prop :=
+  ¬(∃ trg : (RTrigger obs rules), trg.val.active before) ∧ after = []
 
-theorem chaseSequenceSetIsSubsetOfNext (cs : ChaseSequence obs kb) : ∀ n : Nat, cs.fact_sets n ⊆ cs.fact_sets (n+1) := by
-  intro n f h
-  cases cs.triggers_exist n 
-  case inl g =>
-    cases g with | intro trg trgH => 
-      rw [← trgH.right]
-      simp [Set.element, Set.union]
-      apply Or.inr
-      exact h
-  case inr g =>
-    rw [← g.right]
-    simp [Set.element, Set.union]
-    exact h
- 
-theorem chaseSequenceSetIsSubsetOfAllFollowing (cs : ChaseSequence obs kb) : ∀ (n m : Nat), cs.fact_sets n ⊆ cs.fact_sets (n + m) := by
+structure ChaseBranch (obs : ObsoletenessCondition) (kb : KnowledgeBase) where
+  branch : PossiblyInfiniteList FactSet
+  database_first : branch.infinite_list 0 = some kb.db.toFactSet
+  triggers_exist : ∀ n : Nat, (branch.infinite_list n).is_none_or (fun before =>
+    let after := branch.infinite_list (n+1)
+    (exists_trigger_opt_fs obs kb.rules before after) ∨
+    (not_exists_trigger_opt_fs obs kb.rules before after))
+  fairness : ∀ trg : (RTrigger obs kb.rules), ∃ i : Nat, ((branch.infinite_list i).is_some_and (fun fs => ¬ trg.val.active fs))
+    ∧ (∀ j : Nat, j > i -> (branch.infinite_list j).is_none_or (fun fs => ¬ trg.val.active fs))
+
+namespace ChaseBranch
+  def result (branch : ChaseBranch obs kb) : FactSet :=
+    fun f => ∃ n : Nat, (branch.branch.infinite_list n).is_some_and (fun fs => f ∈ fs)
+
+  def terminates (branch : ChaseBranch obs kb) : Prop :=
+    ∃ n : Nat, branch.branch.infinite_list n = none
+end ChaseBranch
+
+structure ChaseTree (obs : ObsoletenessCondition) (kb : KnowledgeBase) where
+  tree : FiniteDegreeTree FactSet
+  database_first : tree.get [] = some kb.db.toFactSet
+  triggers_exist : ∀ node : List Nat, (tree.get node).is_none_or (fun before =>
+    let after := tree.children node
+    (exists_trigger_list obs kb.rules before after) ∨
+    (not_exists_trigger_list obs kb.rules before after))
+
+  fairness_leaves : ∀ leaf, leaf ∈ tree.leaves -> ∀ trg : (RTrigger obs kb.rules), ¬ trg.val.active leaf
+  fairness_infinite_branches : ∀ trg : (RTrigger obs kb.rules), ∃ i : Nat, ∀ node : List Nat, node.length ≥ i ->
+    (tree.get node).is_none_or (fun fs => ¬ trg.val.active fs)
+
+namespace ChaseTree
+  -- NOTE: this does not work; the address might not be valid in the sense that a number might be bigger than the number of disjuncts in a rule head, which leads to malformed branches that are no valid ChaseBranches
+  -- def branch_for (ct : ChaseTree obs kb) (address : InfiniteList Nat) : ChaseBranch obs kb := {
+  --   branch := ct.tree.branch_for address
+  --   database_first := by
+  --     rw [← ct.database_first]
+  --     unfold FiniteDegreeTree.branch_for
+  --     unfold PossiblyInfiniteTree.branch_for
+  --     unfold InfiniteTreeSkeleton.branch_for
+  --     simp
+  --     unfold FiniteDegreeTree.get
+  --     unfold PossiblyInfiniteTree.get
+  --     unfold InfiniteList.take
+  --     rfl
+  --   triggers_exist := by sorry
+  --   fairness := by sorry
+  -- }
+
+  def branches (ct : ChaseTree obs kb) : Set (ChaseBranch obs kb) := fun branch => branch.branch ∈ ct.tree.branches
+
+  def result (ct : ChaseTree obs kb) : Set FactSet := fun fs => ∃ branch, branch ∈ ct.branches ∧ branch.result = fs
+
+  def terminates (ct : ChaseTree obs kb) : Prop := ∀ branch, branch ∈ ct.branches -> branch.terminates
+end ChaseTree
+
+
+theorem chaseBranchSetIsSubsetOfNext (cb : ChaseBranch obs kb) : ∀ n : Nat,
+  match cb.branch.infinite_list n with
+  | .none => cb.branch.infinite_list (n+1) = none
+  | .some fs => (cb.branch.infinite_list (n+1)).is_none_or (fun fs2 => fs ⊆ fs2) :=
+by
+  intro n
+  cases eq : cb.branch.infinite_list n with
+  | none =>
+    simp
+    have dec : Decidable (cb.branch.infinite_list (n+1) = none) := Option.decidable_eq_none
+    apply dec.byContradiction
+    intro contra
+    let n' : Fin (n+1) := ⟨n, by simp⟩
+    have : ¬ cb.branch.infinite_list n' = none := by apply cb.branch.no_holes; apply contra
+    contradiction
+  | some fs =>
+    simp
+    cases eq2 : cb.branch.infinite_list (n+1) with
+    | none => simp [Option.is_none_or]
+    | some fs2 =>
+      simp [Option.is_none_or]
+      intro f h
+      have trg_ex_n := cb.triggers_exist n
+      simp [eq, Option.is_none_or] at trg_ex_n
+      cases trg_ex_n with
+      | inl g =>
+        cases g with | intro trg h_trg =>
+          cases h_trg.right with | intro i h_i =>
+            rw [eq2] at h_i
+            injection h_i with h_i
+            rw [← h_i]
+            simp [Set.element, Set.union]
+            apply Or.inl
+            exact h
+      | inr g =>
+        have g_right := g.right
+        rw [eq2] at g_right
+        contradiction
+
+theorem chaseTreeSetIsSubsetOfEachNext (ct : ChaseTree obs kb) : ∀ address : List Nat,
+  match ct.tree.get address with
+  | .none => ct.tree.children address = []
+  | .some fs => ∀ fs2, fs2 ∈ ct.tree.children address -> fs ⊆ fs2 :=
+by
+  intro address
+  cases eq : ct.tree.get address with
+  | none => simp; apply FiniteDegreeTree.children_empty_when_not_existing; exact eq
+  | some fs =>
+    simp
+    intro fs2 h
+    have trg_ex_addr := ct.triggers_exist address
+    simp [eq, Option.is_none_or] at trg_ex_addr
+    cases trg_ex_addr with
+    | inl g =>
+      cases g with | intro trg h_trg =>
+        rw [← h_trg.right] at h
+        rw [List.mem_map] at h
+        cases h with | intro head h_head =>
+          rw [← h_head.right]
+          intro f h
+          apply Or.inl
+          exact h
+    | inr g =>
+      rw [g.right] at h
+      contradiction
+
+theorem chaseBranchSetIsSubsetOfAllFollowing (cb : ChaseBranch obs kb) : ∀ (n m : Nat),
+  match cb.branch.infinite_list n with
+  | .none => cb.branch.infinite_list (n+m) = none
+  | .some fs => (cb.branch.infinite_list (n+m)).is_none_or (fun fs2 => fs ⊆ fs2) :=
+by
   intro n m
-  induction m
-  simp
-  intro f h 
-  exact h 
-  intro f h 
-  case succ i ih =>
-    apply chaseSequenceSetIsSubsetOfNext cs (n + i)
-    apply ih f
-    exact h 
+  induction m with
+  | zero =>
+    cases eq : cb.branch.infinite_list n with
+    | none => simp; exact eq
+    | some fs => simp [Option.is_none_or, eq, Set.subset]
+  | succ m ih =>
+    cases eq : cb.branch.infinite_list n with
+    | none =>
+      simp
+      simp [eq] at ih
+      have step := chaseBranchSetIsSubsetOfNext cb (n+m)
+      simp [ih] at step
+      exact step
+    | some fs =>
+      simp
+      simp [eq, Option.is_none_or] at ih
+      have step := chaseBranchSetIsSubsetOfNext cb (n+m)
+      cases eq2 : cb.branch.infinite_list (n+m) with
+      | none => simp [eq2] at step; rw [← Nat.add_assoc, step, Option.is_none_or]; simp
+      | some fs2 =>
+        simp [eq2] at step; simp [eq2] at ih; rw [← Nat.add_assoc]
+        cases eq3 : cb.branch.infinite_list (n+m+1) with
+        | none => simp [Option.is_none_or]
+        | some fs3 =>
+          simp [Option.is_none_or]; simp [eq3, Option.is_none_or] at step;
+          apply Set.subsetTransitive; constructor; apply ih; apply step
 
-theorem chaseSequenceSetIsSubsetOfResult (cs : ChaseSequence obs kb) : ∀ n : Nat, cs.fact_sets n ⊆ cs.result := by 
-  intro n 
-  intro e 
-  intro inSet 
+theorem chaseTreeSetIsSubsetOfAllFollowing (ct : ChaseTree obs kb) : ∀ (n m : List Nat),
+  match ct.tree.get n with
+  | .none => ct.tree.get (m ++ n) = none
+  | .some fs => (ct.tree.get (m ++ n)).is_none_or (fun fs2 => fs ⊆ fs2) :=
+by
+  intro n m
+  induction m with
+  | nil =>
+    cases eq : ct.tree.get n with
+    | none => simp; exact eq
+    | some fs => simp [Option.is_none_or, eq, Set.subset]
+  | cons i m ih =>
+    cases eq : ct.tree.get n with
+    | none =>
+      simp
+      simp [eq] at ih
+      have step := chaseTreeSetIsSubsetOfEachNext ct (m ++ n)
+      simp [ih] at step
+      apply FiniteDegreeTree.children_empty_means_all_following_none
+      apply step
+    | some fs =>
+      simp
+      simp [eq, Option.is_none_or] at ih
+      have step := chaseTreeSetIsSubsetOfEachNext ct (m ++ n)
+      cases eq2 : ct.tree.get (m ++ n) with
+      | none =>
+        simp [eq2] at step
+        unfold Option.is_none_or
+        have helper := ct.tree.children_empty_means_all_following_none (m ++ n) step
+        rw [helper]
+        simp
+      | some fs2 =>
+        simp [eq2] at step; simp [eq2] at ih
+        cases eq3 : ct.tree.get (i :: (m ++ n)) with
+        | none => simp [Option.is_none_or]
+        | some fs3 =>
+          simp [Option.is_none_or]
+          apply Set.subsetTransitive
+          constructor
+          apply ih
+          apply step
+
+          rw [ct.tree.in_children_iff_index_exists]
+          exists i
+
+/-
+theorem chaseSequenceSetIsSubsetOfResult (cs : ChaseSequence obs kb) : ∀ n : Nat, cs.fact_sets n ⊆ cs.result := by
+  intro n
+  intro e
+  intro inSet
   simp [ChaseSequence.result, Set.element]
-  exists n 
+  exists n
 
 theorem trgLoadedForChaseResultMeansLoadedAtSomeIndex (cs : ChaseSequence obs kb) : ∀ trg : Trigger obs, trg.loaded cs.result -> ∃ n : Nat, trg.loaded (cs.fact_sets n) := by
-  intro trg 
+  intro trg
   simp [ChaseSequence.result, PreTrigger.loaded]
 
   induction trg.mapped_body
   case nil =>
     intro _
-    exists 0 
-    intro _ contra 
-    contradiction 
+    exists 0
+    intro _ contra
+    contradiction
   case cons head tail ih =>
-    intro loaded 
+    intro loaded
     have ex_head_n := loaded head
     simp [Set.element, List.toSet, Set.union] at ex_head_n
 
-    have ex_tail_n := by 
-      apply ih 
+    have ex_tail_n := by
+      apply ih
       simp [List.toSet] at loaded
-      have ⟨ _, tailSubs ⟩ := (Set.unionSubsetEachSubset _ _ _).mp loaded   
+      have ⟨ _, tailSubs ⟩ := (Set.unionSubsetEachSubset _ _ _).mp loaded
       exact tailSubs
     cases ex_head_n with | intro i hi =>
-      cases ex_tail_n with | intro j hj => 
-        exists Nat.max i j 
+      cases ex_tail_n with | intro j hj =>
+        exists Nat.max i j
         simp [List.toSet]
         rw [Set.unionSubsetEachSubset]
 
-        have max_help_left : ∀ a b : Nat, a ≤ Nat.max a b := by 
+        have max_help_left : ∀ a b : Nat, a ≤ Nat.max a b := by
           intro a b
           simp [Nat.max_def]
-          cases Decidable.em (a ≤ b) 
+          cases Decidable.em (a ≤ b)
           case inl h => simp [h]
           case inr h => simp [h]
-        have max_help_right : ∀ a b : Nat, b ≤ Nat.max a b := by 
+        have max_help_right : ∀ a b : Nat, b ≤ Nat.max a b := by
           intro a b
           simp [Nat.max_def]
-          split -- seems to be the same as the following above: cases Decidable.em (a ≤ b) 
+          split -- seems to be the same as the following above: cases Decidable.em (a ≤ b)
           case isTrue h => simp [h]
           case isFalse h => apply Nat.le_of_lt; apply Nat.lt_of_succ_le; rw [← Nat.not_le_eq]; exact h
         have help_i : i ≤ Nat.max i j := by apply max_help_left
         have help_j : j ≤ Nat.max i j := by apply max_help_right
-        
-        constructor 
+
+        constructor
         apply Set.subsetTransitive _ (cs.fact_sets i) _
-        constructor 
-        intro e he 
-        simp [Set.element] at he 
+        constructor
+        intro e he
+        simp [Set.element] at he
         rw [he]
         assumption
         cases Nat.le.dest help_i with | intro m hm => rw [← hm]; apply chaseSequenceSetIsSubsetOfAllFollowing cs i m
-        cases Nat.le.dest help_j with | intro m hm => 
+        cases Nat.le.dest help_j with | intro m hm =>
           rw [← hm]
           apply Set.subsetTransitive
           constructor
           apply hj
-          apply chaseSequenceSetIsSubsetOfAllFollowing cs j m 
+          apply chaseSequenceSetIsSubsetOfAllFollowing cs j m
 
-theorem trgActiveForChaseResultMeansActiveAtSomeIndex (cs : ChaseSequence obs kb) : ∀ trg : Trigger obs, trg.active cs.result -> ∃ n : Nat, trg.active (cs.fact_sets n) := by 
+theorem trgActiveForChaseResultMeansActiveAtSomeIndex (cs : ChaseSequence obs kb) : ∀ trg : Trigger obs, trg.active cs.result -> ∃ n : Nat, trg.active (cs.fact_sets n) := by
   intro trg
   simp [ChaseSequence.result, Trigger.active]
   intro loaded active
-  have trgLoadedForN := trgLoadedForChaseResultMeansLoadedAtSomeIndex cs trg loaded 
-  cases trgLoadedForN with | intro n loadedN => 
-    exists n 
-    constructor 
+  have trgLoadedForN := trgLoadedForChaseResultMeansLoadedAtSomeIndex cs trg loaded
+  cases trgLoadedForN with | intro n loadedN =>
+    exists n
+    constructor
     exact loadedN
-    intro contra 
+    intro contra
     apply active
     apply obs.monotone
     apply chaseSequenceSetIsSubsetOfResult cs n
     apply contra
 
-theorem funcTermForExisVarInChaseMeansTriggerIsUsed (cs : ChaseSequence obs kb) (trg : RTrigger obs kb.rules) (var : Variable) (i : Nat) : (¬ var ∈ trg.val.rule.frontier) ∧ (∃ f: Fact, f ∈ cs.fact_sets i ∧ ((trg.val.apply_to_var_or_const (VarOrConst.var var)) ∈ f.terms.toSet)) -> ∃ j, j ≤ i ∧ trg.val.result ∪ cs.fact_sets (j-1) = cs.fact_sets j := by 
+theorem funcTermForExisVarInChaseMeansTriggerIsUsed (cs : ChaseSequence obs kb) (trg : RTrigger obs kb.rules) (var : Variable) (i : Nat) : (¬ var ∈ trg.val.rule.frontier) ∧ (∃ f: Fact, f ∈ cs.fact_sets i ∧ ((trg.val.apply_to_var_or_const (VarOrConst.var var)) ∈ f.terms.toSet)) -> ∃ j, j ≤ i ∧ trg.val.result ∪ cs.fact_sets (j-1) = cs.fact_sets j := by
   intro ⟨var_not_in_frontier, exis_f⟩
-  induction i with 
-  | zero => 
+  induction i with
+  | zero =>
     cases exis_f with | intro f hf =>
       let ⟨f_in_db, functional_term_in_f⟩ := hf
       rw [cs.database_first] at f_in_db
-      have : ∀ t, t ≠ GroundSubstitution.apply_skolem_term trg.val.subs (VarOrConst.skolemize trg.val.rule.id (Rule.frontier trg.val.rule) (VarOrConst.var var)) := by 
+      have : ∀ t, t ≠ GroundSubstitution.apply_skolem_term trg.val.subs (VarOrConst.skolemize trg.val.rule.id (Rule.frontier trg.val.rule) (VarOrConst.var var)) := by
         intro t
-        unfold Database.toFactSet at f_in_db 
-        unfold Fact.toFunctionFreeFact at f_in_db 
+        unfold Database.toFactSet at f_in_db
+        unfold Fact.toFunctionFreeFact at f_in_db
         simp only [Set.element] at f_in_db
         split at f_in_db
         case h_1 => contradiction
-        case h_2 _ _ to_fff_is_some =>  
+        case h_2 _ _ to_fff_is_some =>
           split at to_fff_is_some
           case isFalse h => contradiction
           case isTrue _ _ all_terms_ff =>
             have : ¬ (List.all f.terms fun t => match t with
               | GroundTerm.const _ => true
-              | _ => false) = true := by 
+              | _ => false) = true := by
                 apply List.neg_all_of_any_neg
                 apply List.any_of_exists
-                exists GroundSubstitution.apply_skolem_term trg.val.subs (VarOrConst.skolemize trg.val.rule.id (Rule.frontier trg.val.rule) (VarOrConst.var var)) 
+                exists GroundSubstitution.apply_skolem_term trg.val.subs (VarOrConst.skolemize trg.val.rule.id (Rule.frontier trg.val.rule) (VarOrConst.var var))
                 constructor
                 exact functional_term_in_f
                 simp [GroundSubstitution.apply_skolem_term, VarOrConst.skolemize, var_not_in_frontier]
             contradiction
-      apply False.elim 
+      apply False.elim
       apply this
       rfl
   | succ j ih =>
     -- TODO: this should actually be decidable but we need to change the implementation for this
-    cases Classical.em (∃ f: Fact, f ∈ cs.fact_sets j ∧ (trg.val.subs.apply_skolem_term (VarOrConst.skolemize trg.val.rule.id trg.val.rule.frontier (VarOrConst.var var))) ∈ f.terms.toSet) with 
+    cases Classical.em (∃ f: Fact, f ∈ cs.fact_sets j ∧ (trg.val.subs.apply_skolem_term (VarOrConst.skolemize trg.val.rule.id trg.val.rule.frontier (VarOrConst.var var))) ∈ f.terms.toSet) with
     | inl f_in_j =>
       cases ih f_in_j with | intro k hk =>
-        exists k 
+        exists k
         constructor
         apply Nat.le_succ_of_le
         exact hk.left
         exact hk.right
-    | inr f_not_in_j => 
+    | inr f_not_in_j =>
       exists j+1
-      constructor 
+      constructor
       . simp
-      . cases cs.triggers_exist j with 
-        | inr no_trg_ex => 
+      . cases cs.triggers_exist j with
+        | inr no_trg_ex =>
           have : cs.fact_sets j = cs.fact_sets (j+1) := no_trg_ex.right
-          have : ¬ (cs.fact_sets j = cs.fact_sets (j+1)) := by 
-            cases exis_f with | intro f hf => 
-            have : ¬ f ∈ cs.fact_sets j := by 
+          have : ¬ (cs.fact_sets j = cs.fact_sets (j+1)) := by
+            cases exis_f with | intro f hf =>
+            have : ¬ f ∈ cs.fact_sets j := by
               intro f_in_j
               apply f_not_in_j
               exists f
@@ -183,29 +352,29 @@ theorem funcTermForExisVarInChaseMeansTriggerIsUsed (cs : ChaseSequence obs kb) 
               exact f_in_j
               exact hf.right
             have : f ∈ cs.fact_sets (j + 1) := hf.left
-            intro steps_eq 
+            intro steps_eq
             rw [← steps_eq] at this
             contradiction
           contradiction
         | inl trg_ex => cases trg_ex with | intro trg' h_trg' =>
           have : ∃ f, f ∈ PreTrigger.result trg'.val ∧ (trg.val.apply_to_var_or_const (VarOrConst.var var)) ∈ List.toSet f.terms := by
-            cases exis_f with | intro f hf => 
-              exists f 
+            cases exis_f with | intro f hf =>
+              exists f
               constructor
-              . have f_in_next_step := hf.left 
+              . have f_in_next_step := hf.left
                 rw [← h_trg'.right] at f_in_next_step
-                cases f_in_next_step with 
+                cases f_in_next_step with
                 | inl _ => assumption
-                | inr f_in_j => 
+                | inr f_in_j =>
                   apply False.elim
                   apply f_not_in_j
-                  exists f 
-                  constructor 
+                  exists f
+                  constructor
                   exact f_in_j
                   exact hf.right
               . exact hf.right
-          
-          have : ∃ var2, ¬ var2 ∈ trg'.val.rule.frontier ∧ (trg.val.apply_to_var_or_const (VarOrConst.var var)) = (trg'.val.apply_to_var_or_const (VarOrConst.var var2)) := by 
+
+          have : ∃ var2, ¬ var2 ∈ trg'.val.rule.frontier ∧ (trg.val.apply_to_var_or_const (VarOrConst.var var)) = (trg'.val.apply_to_var_or_const (VarOrConst.var var2)) := by
             cases this with | intro f hf =>
               have ⟨f_in_res, apply_var_in_f_terms⟩ := hf
               let i := trg'.val.idx_of_fact_in_result f f_in_res
@@ -214,39 +383,39 @@ theorem funcTermForExisVarInChaseMeansTriggerIsUsed (cs : ChaseSequence obs kb) 
               cases List.inToSetMeansExistsIndex _ _ apply_var_in_f_terms with | intro k hk =>
                 have f_is_at_its_idx : f = trg'.val.mapped_head.get ⟨i.val, by simp [PreTrigger.mapped_head]⟩ := by simp [i, PreTrigger.idx_of_fact_in_result]; apply List.idx_of_get
 
-                have atom_arity_same_as_fact : f.terms.length = List.length (FunctionFreeAtom.terms atom_for_f) := by 
+                have atom_arity_same_as_fact : f.terms.length = List.length (FunctionFreeAtom.terms atom_for_f) := by
                   rw [f_is_at_its_idx]
                   unfold PreTrigger.mapped_head
                   unfold PreTrigger.apply_to_function_free_atom
                   simp [atom_for_f]
 
-                let term_for_f := atom_for_f.terms.get ⟨k.val, (by 
+                let term_for_f := atom_for_f.terms.get ⟨k.val, (by
                   rw [← atom_arity_same_as_fact]
                   exact k.isLt
                 )⟩
 
                 -- TODO: this is similar to stuff going on around line 590; check if we can unify
-                have : (trg'.val.apply_to_var_or_const term_for_f) = f.terms.get k := by 
+                have : (trg'.val.apply_to_var_or_const term_for_f) = f.terms.get k := by
                   have : f.terms = (trg'.val.apply_to_function_free_atom atom_for_f).terms := by
                     conv => lhs; rw [f_is_at_its_idx]
                     rw [← PreTrigger.apply_subs_to_atom_at_idx_same_as_fact_at_idx]
                   rw [List.get_eq_of_eq this]
                   simp [PreTrigger.apply_to_function_free_atom, term_for_f]
 
-                have : (trg.val.apply_to_var_or_const (VarOrConst.var var)) = (trg'.val.apply_to_var_or_const term_for_f) := by 
+                have : (trg.val.apply_to_var_or_const (VarOrConst.var var)) = (trg'.val.apply_to_var_or_const term_for_f) := by
                   rw [← this] at hk
                   exact hk
 
-                cases eq_term_for_f : term_for_f with 
-                | const c => 
+                cases eq_term_for_f : term_for_f with
+                | const c =>
                   rw [eq_term_for_f] at this
                   simp [PreTrigger.apply_to_var_or_const, PreTrigger.apply_to_skolemized_term, PreTrigger.skolemize_var_or_const, GroundSubstitution.apply_skolem_term, VarOrConst.skolemize, var_not_in_frontier] at this
                   contradiction
                 | var var_for_f =>
                   exists var_for_f
-                  have var_for_f_not_in_frontier : ¬ var_for_f ∈ trg'.val.rule.frontier := by 
+                  have var_for_f_not_in_frontier : ¬ var_for_f ∈ trg'.val.rule.frontier := by
                     apply Decidable.byContradiction
-                    intro h 
+                    intro h
                     simp at h
                     rw [eq_term_for_f] at this
 
@@ -254,7 +423,7 @@ theorem funcTermForExisVarInChaseMeansTriggerIsUsed (cs : ChaseSequence obs kb) 
                     have var_for_f_occurs_in_body_atom := trg'.val.rule.frontier_var_occurs_in_fact_in_body var_for_f h
                     cases var_for_f_occurs_in_body_atom with | intro body_atom_for_f h_body_atom_for_f =>
                       exists (SubsTarget.apply trg'.val.subs body_atom_for_f)
-                      constructor 
+                      constructor
                       . have trg'_loaded := h_trg'.left.left
                         apply trg'_loaded
                         unfold PreTrigger.mapped_body
@@ -279,13 +448,13 @@ theorem funcTermForExisVarInChaseMeansTriggerIsUsed (cs : ChaseSequence obs kb) 
                   . rw [eq_term_for_f] at this
                     exact this
 
-          have : trg.val.rule = trg'.val.rule ∧ ∀ v, v ∈ trg.val.rule.frontier.toSet -> trg.val.subs v = trg'.val.subs v := by 
+          have : trg.val.rule = trg'.val.rule ∧ ∀ v, v ∈ trg.val.rule.frontier.toSet -> trg.val.subs v = trg'.val.subs v := by
             cases this with | intro var2 hvar2 =>
               apply RTrigger.funcTermForExisVarInMultipleTriggersMeansTheyAreTheSame
               apply var_not_in_frontier
               apply hvar2.left
               apply hvar2.right
-          have : trg.val.mapped_head = trg'.val.mapped_head := by 
+          have : trg.val.mapped_head = trg'.val.mapped_head := by
             unfold PreTrigger.mapped_head
             rw [← this.left]
             apply List.map_eq_map_if_functions_eq
@@ -293,18 +462,18 @@ theorem funcTermForExisVarInChaseMeansTriggerIsUsed (cs : ChaseSequence obs kb) 
             unfold PreTrigger.apply_to_function_free_atom
             simp
             intro voc hvoc
-            cases voc with 
-            | const c => simp [PreTrigger.apply_to_var_or_const, PreTrigger.apply_to_skolemized_term, PreTrigger.skolemize_var_or_const, GroundSubstitution.apply_skolem_term, VarOrConst.skolemize] 
+            cases voc with
+            | const c => simp [PreTrigger.apply_to_var_or_const, PreTrigger.apply_to_skolemized_term, PreTrigger.skolemize_var_or_const, GroundSubstitution.apply_skolem_term, VarOrConst.skolemize]
             | var v =>
-              cases Decidable.em (v ∈ trg.val.rule.frontier) with 
-              | inl v_in_frontier => 
+              cases Decidable.em (v ∈ trg.val.rule.frontier) with
+              | inl v_in_frontier =>
                 simp [PreTrigger.apply_to_var_or_const, PreTrigger.apply_to_skolemized_term, PreTrigger.skolemize_var_or_const, GroundSubstitution.apply_skolem_term]
                 rw [← this.left]
                 simp [VarOrConst.skolemize, v_in_frontier]
                 apply this.right
                 apply List.listElementAlsoToSetElement
                 apply v_in_frontier
-              | inr v_not_in_frontier => 
+              | inr v_not_in_frontier =>
                 simp [PreTrigger.apply_to_var_or_const, PreTrigger.apply_to_skolemized_term, PreTrigger.skolemize_var_or_const, GroundSubstitution.apply_skolem_term]
                 rw [← this.left]
                 simp [VarOrConst.skolemize, v_not_in_frontier]
@@ -315,16 +484,16 @@ theorem funcTermForExisVarInChaseMeansTriggerIsUsed (cs : ChaseSequence obs kb) 
                 rw [← this.right w]
                 exact hw
 
-          have : trg.val.result = trg'.val.result := by 
-            unfold PreTrigger.result 
+          have : trg.val.result = trg'.val.result := by
+            unfold PreTrigger.result
             rw [this]
           rw [this]
           exact h_trg'.right
 
-theorem funcTermForExisVarInChaseMeansTriggerResultOccurs (cs : ChaseSequence obs kb) (trg : RTrigger obs kb.rules) (var : Variable) (i : Nat) : (¬ var ∈ trg.val.rule.frontier) ∧ (∃ f: Fact, f ∈ cs.fact_sets i ∧ (trg.val.apply_to_var_or_const (VarOrConst.var var)) ∈ f.terms.toSet) -> trg.val.result ⊆ cs.fact_sets i := by 
-  intro h 
+theorem funcTermForExisVarInChaseMeansTriggerResultOccurs (cs : ChaseSequence obs kb) (trg : RTrigger obs kb.rules) (var : Variable) (i : Nat) : (¬ var ∈ trg.val.rule.frontier) ∧ (∃ f: Fact, f ∈ cs.fact_sets i ∧ (trg.val.apply_to_var_or_const (VarOrConst.var var)) ∈ f.terms.toSet) -> trg.val.result ⊆ cs.fact_sets i := by
+  intro h
   cases funcTermForExisVarInChaseMeansTriggerIsUsed cs trg var i h with | intro j hj =>
-    have : trg.val.result ⊆ cs.fact_sets j := by 
+    have : trg.val.result ⊆ cs.fact_sets j := by
       rw [← hj.right]
       apply Set.subsetUnionSomethingStillSubset
       apply Set.subsetOfSelf
@@ -332,7 +501,7 @@ theorem funcTermForExisVarInChaseMeansTriggerResultOccurs (cs : ChaseSequence ob
     apply Set.subsetTransitive
     constructor
     apply this
-    cases Nat.le.dest hj.left with | intro k hk => 
+    cases Nat.le.dest hj.left with | intro k hk =>
       rw [← hk]
       apply chaseSequenceSetIsSubsetOfAllFollowing
 
@@ -345,26 +514,26 @@ namespace KnowledgeBase
 end KnowledgeBase
 
 noncomputable def inductive_homomorphism (cs : ChaseSequence obs kb) (m : FactSet) (mIsModel : m.modelsKb obs kb) : (i : Nat) -> { hom : GroundTermMapping // isHomomorphism hom (cs.fact_sets i) m }
-| .zero => ⟨id, (by 
-  constructor 
+| .zero => ⟨id, (by
+  constructor
   . unfold isIdOnConstants ; intro gt ; cases gt <;> simp
   . rw [cs.database_first]
-    intro el 
+    intro el
     simp [Set.element]
-    intro elInSet 
-    cases elInSet with | intro f hf => 
+    intro elInSet
+    cases elInSet with | intro f hf =>
       apply mIsModel.left
-      simp [Set.element] 
+      simp [Set.element]
       have : f = el := by have hfr := hf.right; simp [applyFact, List.map_id'] at hfr; exact hfr
       rw [this] at hf
       exact hf.left
-)⟩ 
-| .succ j => 
+)⟩
+| .succ j =>
   let prev_hom := inductive_homomorphism cs m mIsModel j
 
   let trg_ex_dec := Classical.propDecidable (∃ trg : (RTrigger obs kb.rules), trg.val.active (cs.fact_sets j) ∧ trg.val.result ∪ cs.fact_sets j = cs.fact_sets (j + 1))
-  match trg_ex_dec with 
-  | .isFalse n_trg_ex => ⟨prev_hom.val, (by 
+  match trg_ex_dec with
+  | .isFalse n_trg_ex => ⟨prev_hom.val, (by
     have sequence_finished := by cases cs.triggers_exist j with
     | inl _ => contradiction
     | inr hr => exact hr
@@ -382,34 +551,34 @@ noncomputable def inductive_homomorphism (cs : ChaseSequence obs kb) (m : FactSe
       }
       property := trg.property
     }
-    have trg_variant_loaded_for_m : trg_variant_for_m.val.loaded m := by 
-      have : trg_variant_for_m.val.loaded (applyFactSet prev_hom (cs.fact_sets j)) := by 
+    have trg_variant_loaded_for_m : trg_variant_for_m.val.loaded m := by
+      have : trg_variant_for_m.val.loaded (applyFactSet prev_hom (cs.fact_sets j)) := by
         apply PreTrigger.term_mapping_preserves_loadedness
         exact prev_hom.property.left
         exact trg_active_for_current_step.left
       apply Set.subsetTransitive
       exact ⟨this, prev_hom.property.right⟩
-    have trg_variant_obsolete_on_m : obs.cond trg_variant_for_m.val m := by 
-      have m_models_trg : m.modelsRule obs trg_variant_for_m.val.rule := by exact mIsModel.right trg.val.rule trg.property 
+    have trg_variant_obsolete_on_m : obs.cond trg_variant_for_m.val m := by
+      have m_models_trg : m.modelsRule obs trg_variant_for_m.val.rule := by exact mIsModel.right trg.val.rule trg.property
       unfold FactSet.modelsRule at m_models_trg
       apply m_models_trg
       constructor
-      rfl 
+      rfl
       apply trg_variant_loaded_for_m
 
     let obs_for_m_subs := Classical.choose (obs.cond_implies_trg_is_satisfied trg_variant_obsolete_on_m)
     let h_obs_for_m_subs := Classical.choose_spec (obs.cond_implies_trg_is_satisfied trg_variant_obsolete_on_m)
 
     let next_hom : GroundTermMapping := fun t =>
-      match t with 
+      match t with
       | FiniteTree.leaf _ => t
       | FiniteTree.inner _ _ =>
         let t_in_step_j_dec := Classical.propDecidable (∃ f, f ∈ (cs.fact_sets j) ∧ t ∈ f.terms.toSet)
-        match t_in_step_j_dec with 
+        match t_in_step_j_dec with
         | Decidable.isTrue _ => prev_hom.val t
         | Decidable.isFalse _ =>
           let t_in_trg_result_dec := Classical.propDecidable (∃ f, f ∈ trg.val.result ∧ t ∈ f.terms.toSet)
-          match t_in_trg_result_dec with 
+          match t_in_trg_result_dec with
           | Decidable.isFalse _ => t
           | Decidable.isTrue t_in_trg_result =>
             let f := Classical.choose t_in_trg_result
@@ -421,24 +590,24 @@ noncomputable def inductive_homomorphism (cs : ChaseSequence obs kb) (m : FactSe
             have idx_t_in_f_isLt := idx_t_in_f.isLt
             have f_is_at_its_idx : f = trg.val.mapped_head.get ⟨idx_f.val, by simp [PreTrigger.mapped_head]⟩ := by simp [idx_f, PreTrigger.idx_of_fact_in_result]; apply List.idx_of_get
 
-            have atom_arity_same_as_fact : f.terms.length = List.length (FunctionFreeAtom.terms atom_in_head) := by 
+            have atom_arity_same_as_fact : f.terms.length = List.length (FunctionFreeAtom.terms atom_in_head) := by
                 rw [f_is_at_its_idx]
                 unfold PreTrigger.mapped_head
                 unfold PreTrigger.apply_to_function_free_atom
                 simp [atom_in_head]
 
-            let term_corresponding_to_t := atom_in_head.terms.get ⟨idx_t_in_f.val, (by 
+            let term_corresponding_to_t := atom_in_head.terms.get ⟨idx_t_in_f.val, (by
               rw [← atom_arity_same_as_fact]
               exact idx_t_in_f_isLt
             )⟩
 
             obs_for_m_subs.apply_var_or_const term_corresponding_to_t
 
-    ⟨next_hom, (by 
-      constructor 
-      . intro term 
-        split 
-        . simp 
+    ⟨next_hom, (by
+      constructor
+      . intro term
+        split
+        . simp
         . trivial
       . rw [← trg_result_used_for_next_chase_step]
         intro mapped_fact fact_in_chase
@@ -446,30 +615,30 @@ noncomputable def inductive_homomorphism (cs : ChaseSequence obs kb) (m : FactSe
         cases fact_in_chase with | intro fact fact_in_chase =>
           rw [← fact_in_chase.right]
           let fact_in_chase := fact_in_chase.left
-           
-          cases fact_in_chase with 
-          | inr fact_in_prev_step => 
-            apply prev_hom.property.right 
+
+          cases fact_in_chase with
+          | inr fact_in_prev_step =>
+            apply prev_hom.property.right
             exists fact
             constructor
-            exact fact_in_prev_step 
+            exact fact_in_prev_step
             unfold applyFact
             simp
             intro ground_term _
-            have : ∃ f, f ∈ (cs.fact_sets j) ∧ ground_term ∈ f.terms.toSet := by 
+            have : ∃ f, f ∈ (cs.fact_sets j) ∧ ground_term ∈ f.terms.toSet := by
               exists fact
               rw [← List.listElementIffToSetElement]
               constructor
               assumption
               assumption
-            cases ground_term with 
+            cases ground_term with
             | leaf c => simp [next_hom]; apply prev_hom.property.left (GroundTerm.const c)
-            | inner _ _ => 
-              simp [next_hom] 
+            | inner _ _ =>
+              simp [next_hom]
               split
               . rfl
               . contradiction
-          | inl fact_in_trg_result => 
+          | inl fact_in_trg_result =>
             let idx_of_fact_in_result := trg.val.idx_of_fact_in_result fact fact_in_trg_result
             have fact_is_at_its_idx : fact = trg.val.mapped_head.get ⟨idx_of_fact_in_result.val, by simp [PreTrigger.mapped_head]⟩ := by simp [idx_of_fact_in_result, PreTrigger.idx_of_fact_in_result]; apply List.idx_of_get
 
@@ -478,19 +647,19 @@ noncomputable def inductive_homomorphism (cs : ChaseSequence obs kb) (m : FactSe
 
             apply h_obs_for_m_subs.right
             apply List.existsIndexMeansInToSet
-            exists ⟨idx_of_fact_in_result.val, (by simp [GroundSubstitution.apply_function_free_conj])⟩ 
+            exists ⟨idx_of_fact_in_result.val, (by simp [GroundSubstitution.apply_function_free_conj])⟩
             simp [GroundSubstitution.apply_function_free_conj, GroundSubstitution.apply_function_free_atom, PreTrigger.mapped_head, PreTrigger.apply_to_function_free_atom]
 
             -- we show that applying next_hom after trg is the same is applying trg_variant_for_m for each relevant VarOrConst
 
-            intro voc voc_is_in_head_atom_for_fact 
-            cases voc with 
+            intro voc voc_is_in_head_atom_for_fact
+            cases voc with
             | const _ => simp [PreTrigger.apply_to_var_or_const, PreTrigger.apply_to_skolemized_term, PreTrigger.skolemize_var_or_const, VarOrConst.skolemize, GroundSubstitution.apply_skolem_term, GroundSubstitution.apply_var_or_const]
-            | var v_from_head_atom => 
+            | var v_from_head_atom =>
               simp [next_hom, GroundSubstitution.apply_skolem_term, GroundSubstitution.apply_var_or_const]
-              split 
+              split
               case h_1 c h_c_eq =>
-                have v_is_in_frontier : v_from_head_atom ∈ trg.val.rule.frontier := by 
+                have v_is_in_frontier : v_from_head_atom ∈ trg.val.rule.frontier := by
                   apply Decidable.byContradiction
                   intro opp
                   simp [PreTrigger.apply_to_var_or_const, PreTrigger.apply_to_skolemized_term, PreTrigger.skolemize_var_or_const, GroundSubstitution.apply_skolem_term, VarOrConst.skolemize, opp] at h_c_eq
@@ -501,15 +670,15 @@ noncomputable def inductive_homomorphism (cs : ChaseSequence obs kb) (m : FactSe
                 have prev_hom_id_on_constants := prev_hom.property.left (FiniteTree.leaf c)
                 simp at prev_hom_id_on_constants
                 rw [prev_hom_id_on_constants]
-              case h_2 => 
-                split 
-                case h_1 _ exis_f _ => 
-                  have v_is_in_frontier : v_from_head_atom ∈ trg.val.rule.frontier := by 
+              case h_2 =>
+                split
+                case h_1 _ exis_f _ =>
+                  have v_is_in_frontier : v_from_head_atom ∈ trg.val.rule.frontier := by
                     apply Decidable.byContradiction
                     intro v_not_in_frontier
                     simp at v_not_in_frontier
 
-                    have : trg.val.result ⊆ cs.fact_sets j := by 
+                    have : trg.val.result ⊆ cs.fact_sets j := by
                       apply funcTermForExisVarInChaseMeansTriggerResultOccurs
                       constructor
                       apply v_not_in_frontier
@@ -525,14 +694,14 @@ noncomputable def inductive_homomorphism (cs : ChaseSequence obs kb) (m : FactSe
                   have : trg.val.rule = trg_variant_for_m.val.rule := by rfl
                   rw [← this]
                   apply v_is_in_frontier
-                case h_2 _ n_exis_f_for_step_j _ => 
-                  have v_not_in_frontier : ¬ v_from_head_atom ∈ trg.val.rule.frontier := by 
+                case h_2 _ n_exis_f_for_step_j _ =>
+                  have v_not_in_frontier : ¬ v_from_head_atom ∈ trg.val.rule.frontier := by
                     intro v_is_in_frontier
                     have v_in_body := Rule.frontier_var_occurs_in_fact_in_body _ _ v_is_in_frontier
                     cases v_in_body with | intro f hf =>
                       apply n_exis_f_for_step_j
                       exists (trg.val.subs.apply_function_free_atom f)
-                      constructor 
+                      constructor
                       . apply trg_active_for_current_step.left
                         unfold PreTrigger.mapped_body
                         apply List.mappedElemInMappedList
@@ -542,13 +711,13 @@ noncomputable def inductive_homomorphism (cs : ChaseSequence obs kb) (m : FactSe
                         rw [this]
                         apply List.mappedElemInMappedList
                         apply hf.right
-                  split 
-                  case h_1 _ n_exis_f_for_trg_result _ => 
-                    apply False.elim 
+                  split
+                  case h_1 _ n_exis_f_for_trg_result _ =>
+                    apply False.elim
                     apply n_exis_f_for_trg_result
                     exists fact
-                    constructor 
-                    exact fact_in_trg_result 
+                    constructor
+                    exact fact_in_trg_result
                     rw [fact_is_at_its_idx]
 
                     rw [← PreTrigger.apply_subs_to_atom_at_idx_same_as_fact_at_idx]
@@ -556,14 +725,14 @@ noncomputable def inductive_homomorphism (cs : ChaseSequence obs kb) (m : FactSe
                     apply List.existsIndexMeansInToSet
                     rw [List.listElementIffToSetElement] at voc_is_in_head_atom_for_fact
                     cases (List.inToSetMeansExistsIndex _ _ voc_is_in_head_atom_for_fact) with | intro voc_idx h_voc_idx =>
-                      exists ⟨voc_idx.val, (by 
+                      exists ⟨voc_idx.val, (by
                         rw [← PreTrigger.apply_to_function_free_atom_terms_same_length]
                         apply voc_idx.isLt
                       )⟩
                       simp [GroundSubstitution.apply_atom, VarOrConst.skolemize, GroundSubstitution.apply_skolem_term, FunctionFreeAtom.skolemize, PreTrigger.apply_to_function_free_atom, PreTrigger.apply_to_var_or_const, PreTrigger.apply_to_skolemized_term, PreTrigger.skolemize_var_or_const]
                       simp at h_voc_idx
                       rw [← h_voc_idx]
-                  case h_2 _ exis_f _ => 
+                  case h_2 _ exis_f _ =>
                     split
                     case _ _ chosen_f_in_result applied_v_is_in_chosen_f _ =>
 
@@ -578,24 +747,24 @@ noncomputable def inductive_homomorphism (cs : ChaseSequence obs kb) (m : FactSe
                       have f_is_at_its_idx : chosen_f = trg.val.mapped_head.get ⟨idx_f.val, by simp [PreTrigger.mapped_head]⟩ := by simp [idx_f, PreTrigger.idx_of_fact_in_result]; apply List.idx_of_get
                       have v_is_at_its_idx : (trg.val.apply_to_var_or_const v_from_head_atom) = chosen_f.terms.get idx_v_in_f := by simp [idx_v_in_f]; apply List.idx_of_get
 
-                      have atom_arity_same_as_fact : chosen_f.terms.length = List.length (FunctionFreeAtom.terms atom_in_head) := by 
+                      have atom_arity_same_as_fact : chosen_f.terms.length = List.length (FunctionFreeAtom.terms atom_in_head) := by
                         rw [f_is_at_its_idx]
                         unfold PreTrigger.mapped_head
                         simp
                         rw [← PreTrigger.apply_to_function_free_atom_terms_same_length]
                         simp [atom_in_head]
 
-                      let var_corresponding_to_applied_v := atom_in_head.terms.get ⟨idx_v_in_f.val, (by 
+                      let var_corresponding_to_applied_v := atom_in_head.terms.get ⟨idx_v_in_f.val, (by
                         rw [← atom_arity_same_as_fact]
                         exact idx_v_in_f_isLt
                       )⟩
 
                       let skolem_term_corresponding_to_applied_v := trg.val.skolemize_var_or_const var_corresponding_to_applied_v
 
-                      have subs_application_is_injective_for_freshly_introduced_terms : ∀ s, trg.val.apply_to_skolemized_term skolem_v = trg.val.apply_to_var_or_const s -> skolem_v = trg.val.skolemize_var_or_const s := by 
+                      have subs_application_is_injective_for_freshly_introduced_terms : ∀ s, trg.val.apply_to_skolemized_term skolem_v = trg.val.apply_to_var_or_const s -> skolem_v = trg.val.skolemize_var_or_const s := by
                         intro s hs
-                        cases s with 
-                        | const const_s => 
+                        cases s with
+                        | const const_s =>
                           simp [skolem_v, PreTrigger.apply_to_var_or_const, PreTrigger.apply_to_skolemized_term, PreTrigger.skolemize_var_or_const, VarOrConst.skolemize, v_not_in_frontier, GroundSubstitution.apply_skolem_term] at hs
                           contradiction
                         | var var_s =>
@@ -603,20 +772,20 @@ noncomputable def inductive_homomorphism (cs : ChaseSequence obs kb) (m : FactSe
                           apply v_not_in_frontier
                           apply hs
 
-                      have skolemized_ts_are_equal : skolem_term_corresponding_to_applied_v = skolem_v := by 
-                        apply Eq.symm 
+                      have skolemized_ts_are_equal : skolem_term_corresponding_to_applied_v = skolem_v := by
+                        apply Eq.symm
                         apply subs_application_is_injective_for_freshly_introduced_terms
                         unfold PreTrigger.apply_to_var_or_const at v_is_at_its_idx
                         simp at v_is_at_its_idx
                         rw [v_is_at_its_idx]
 
-                        have : chosen_f.terms = (trg.val.apply_to_function_free_atom atom_in_head).terms := by 
+                        have : chosen_f.terms = (trg.val.apply_to_function_free_atom atom_in_head).terms := by
                           rw [f_is_at_its_idx]
                           rw [← PreTrigger.apply_subs_to_atom_at_idx_same_as_fact_at_idx]
 
                         simp [this, PreTrigger.apply_to_function_free_atom, var_corresponding_to_applied_v]
 
-                      have : var_corresponding_to_applied_v = v_from_head_atom := by 
+                      have : var_corresponding_to_applied_v = v_from_head_atom := by
                         apply VarOrConst.skolemize_injective trg.val.rule.id (Rule.frontier trg.val.rule)
                         apply skolemized_ts_are_equal
 
@@ -625,7 +794,7 @@ noncomputable def inductive_homomorphism (cs : ChaseSequence obs kb) (m : FactSe
 
     )⟩
 
-theorem inductive_homomorphism_same_on_terms_in_next_step (cs : ChaseSequence obs kb) (m : FactSet) (mIsModel : m.modelsKb obs kb) : ∀ i f t, f ∈ cs.fact_sets i ∧ t ∈ f.terms.toSet -> (inductive_homomorphism cs m mIsModel i).val t = (inductive_homomorphism cs m mIsModel (Nat.succ i)).val t := by 
+theorem inductive_homomorphism_same_on_terms_in_next_step (cs : ChaseSequence obs kb) (m : FactSet) (mIsModel : m.modelsKb obs kb) : ∀ i f t, f ∈ cs.fact_sets i ∧ t ∈ f.terms.toSet -> (inductive_homomorphism cs m mIsModel i).val t = (inductive_homomorphism cs m mIsModel (Nat.succ i)).val t := by
   intro i f t ⟨f_in_step_i, t_is_term_in_f⟩
   conv =>
     rhs
@@ -633,21 +802,21 @@ theorem inductive_homomorphism_same_on_terms_in_next_step (cs : ChaseSequence ob
     simp
   split
   case h_1 _ n_ex_trg _ => simp [n_ex_trg]
-  case h_2 _ _ _ => 
+  case h_2 _ _ _ =>
     split
     simp
     split
     case h_1 c => exact (inductive_homomorphism cs m mIsModel i).property.left (GroundTerm.const c)
-    case h_2 ft => 
-      split 
+    case h_2 ft =>
+      split
       case h_1 _ ex_f _ => rfl
       case h_2 _ n_ex_f _ => apply False.elim; apply n_ex_f; exists f
 
-theorem inductive_homomorphism_same_on_all_following_terms (cs : ChaseSequence obs kb) (m : FactSet) (mIsModel : m.modelsKb obs kb) : ∀ i j f t, f ∈ cs.fact_sets i ∧ t ∈ f.terms.toSet -> (inductive_homomorphism cs m mIsModel i).val t = (inductive_homomorphism cs m mIsModel (i + j)).val t := by 
+theorem inductive_homomorphism_same_on_all_following_terms (cs : ChaseSequence obs kb) (m : FactSet) (mIsModel : m.modelsKb obs kb) : ∀ i j f t, f ∈ cs.fact_sets i ∧ t ∈ f.terms.toSet -> (inductive_homomorphism cs m mIsModel i).val t = (inductive_homomorphism cs m mIsModel (i + j)).val t := by
   intro i j f t
-  induction j with 
+  induction j with
   | zero => intros; rfl
-  | succ k ih => 
+  | succ k ih =>
     intro h_precondition
     rw [ih h_precondition]
     apply inductive_homomorphism_same_on_terms_in_next_step
@@ -661,77 +830,77 @@ theorem chaseResultUnivModelsKb (cs : ChaseSequence obs kb) : cs.result.universa
   constructor
 
   -- DB in CS
-  unfold FactSet.modelsDb 
+  unfold FactSet.modelsDb
   unfold ChaseSequence.result
-  intro f 
-  intro h 
+  intro f
+  intro h
   exists 0
   rw [cs.database_first]
   exact h
-  
+
   -- Rules modelled
   unfold FactSet.modelsRules
-  intro r 
-  intro h 
+  intro r
+  intro h
   unfold FactSet.modelsRule
   simp
   intro trg trg_rule trg_loaded
   apply Classical.byContradiction
   intro trg_not_obsolete
-  cases (trgActiveForChaseResultMeansActiveAtSomeIndex cs trg ⟨trg_loaded, trg_not_obsolete⟩) with | intro i active_i => 
-    have not_active_eventually := cs.fairness ⟨trg, by rw [← trg_rule] at h; apply h⟩ i active_i 
-    cases not_active_eventually with | intro j not_active_j => 
-      have ⟨j_ge_i, not_active_j⟩ := not_active_j 
+  cases (trgActiveForChaseResultMeansActiveAtSomeIndex cs trg ⟨trg_loaded, trg_not_obsolete⟩) with | intro i active_i =>
+    have not_active_eventually := cs.fairness ⟨trg, by rw [← trg_rule] at h; apply h⟩ i active_i
+    cases not_active_eventually with | intro j not_active_j =>
+      have ⟨j_ge_i, not_active_j⟩ := not_active_j
       simp [Trigger.active] at not_active_j
-      have obsolete_j := not_active_j (by 
-        simp [PreTrigger.loaded] 
-        apply Set.subsetTransitive 
-        constructor 
-        apply active_i.left 
+      have obsolete_j := not_active_j (by
+        simp [PreTrigger.loaded]
+        apply Set.subsetTransitive
+        constructor
+        apply active_i.left
         cases Nat.le.dest j_ge_i with | intro m hm => rw [← hm]; apply chaseSequenceSetIsSubsetOfAllFollowing cs i m
       )
       apply trg_not_obsolete
       apply obs.monotone
       apply chaseSequenceSetIsSubsetOfResult cs j
       apply obsolete_j
-  
+
   -- universality
   intro m mIsModel
 
   let inductive_homomorphism_shortcut := inductive_homomorphism cs m mIsModel
 
-  let global_h : GroundTermMapping := fun t => 
+  let global_h : GroundTermMapping := fun t =>
     let dec := Classical.propDecidable (∃ f, f ∈ cs.result ∧ t ∈ f.terms.toSet)
     match dec with
-      | Decidable.isTrue p => 
+      | Decidable.isTrue p =>
         let ⟨hfl, _⟩ := Classical.choose_spec p
         let i := Classical.choose hfl
         let target_h := inductive_homomorphism_shortcut i
         target_h.val t
       | Decidable.isFalse _ => t
 
-  have : ∀ i f, f ∈ cs.fact_sets i -> applyFact global_h f = applyFact (inductive_homomorphism_shortcut i).val f := by 
+  have : ∀ i f, f ∈ cs.fact_sets i -> applyFact global_h f = applyFact (inductive_homomorphism_shortcut i).val f := by
     intro i f f_in_step_i
     unfold applyFact
     simp [global_h]
     -- apply List.map_eq_map_if_functions_eq
     intro t t_is_term_in_f
-    split 
-    case h_2 _ n_ex_f' _ => 
-      apply False.elim 
-      apply n_ex_f' 
-      exists f 
-      constructor 
+    split
+    case h_2 _ n_ex_f' _ =>
+      apply False.elim
+      apply n_ex_f'
+      exists f
+      constructor
       . apply chaseSequenceSetIsSubsetOfResult; apply f_in_step_i
       . rw [← List.listElementIffToSetElement]; apply t_is_term_in_f
-    case h_1 _ ex_f' _ => 
+    case h_1 _ ex_f' _ =>
       split
-      case _ f' t_is_term_in_f' _ => 
+      case _ f' t_is_term_in_f' _ =>
         let j := Classical.choose f'
         let f'_in_step_j := Classical.choose_spec f'
         cases Nat.le_total i j with
-        | inl i_le_j => 
-          have j_is_i_plus_k := Nat.le.dest i_le_j 
+        | inl i_le_j =>
+          have j_is_i_plus_k := Nat.le.dest i_le_j
           cases j_is_i_plus_k with | intro k hk =>
             simp [j] at hk
             rw [← hk]
@@ -740,25 +909,25 @@ theorem chaseResultUnivModelsKb (cs : ChaseSequence obs kb) : cs.result.universa
             constructor
             apply f_in_step_i
             rw [← List.listElementIffToSetElement]; apply t_is_term_in_f
-        | inr j_le_i => 
-          have i_is_j_plus_k := Nat.le.dest j_le_i 
+        | inr j_le_i =>
+          have i_is_j_plus_k := Nat.le.dest j_le_i
           cases i_is_j_plus_k with | intro k hk =>
             rw [← hk]
             apply inductive_homomorphism_same_on_all_following_terms
             constructor
             apply f'_in_step_j
             apply t_is_term_in_f'
-  
+
   exists global_h
   constructor
-  . intro gt 
-    split 
-    case h_1 _ c => 
+  . intro gt
+    split
+    case h_1 _ c =>
       simp [global_h]
-      split 
-      . split 
-        case h_1 hfl _ _ => 
-          let i := Classical.choose hfl 
+      split
+      . split
+        case h_1 hfl _ _ =>
+          let i := Classical.choose hfl
           exact (inductive_homomorphism_shortcut i).property.left (GroundTerm.const c)
       . trivial
     . trivial
@@ -768,7 +937,7 @@ theorem chaseResultUnivModelsKb (cs : ChaseSequence obs kb) : cs.result.universa
     unfold Set.element at hf
     unfold applyFactSet at hf
     cases hf with | intro e he =>
-      let ⟨hel, her⟩ := he 
+      let ⟨hel, her⟩ := he
       simp [Set.element] at hel
       cases hel with | intro n hn =>
         rw [← her]
@@ -778,4 +947,5 @@ theorem chaseResultUnivModelsKb (cs : ChaseSequence obs kb) : cs.result.universa
         apply this
         simp [Set.element, applyFactSet]
         exists e
+-/
 
