ProofLibrary/PossiblyInfiniteList.lean
@@ -1,7 +1,55 @@
 -- import Mathlib.Data.Stream.Defs
+import ProofLibrary.List
 
-def Stream' (α : Type u) := Nat -> α 
+def InfiniteList (α : Type u) := Nat -> α 
 
-structure PossiblyInfiniteList (α) where
-  infinite_list : Stream' (Option α)
-  no_holes : ∀ n : Nat, infinite_list n ≠ none -> ∀ m : Nat, m < n -> infinite_list m ≠ none
+namespace InfiniteList
+  def take (l : InfiniteList α) : Nat -> List α
+  | 0 => []
+  | n+1 => (l.take n) ++ [l (n+1)]
+
+  def skip (l : InfiniteList α) (m : Nat) : InfiniteList α := fun n => l (n + m)
+
+  theorem skip_zero_eq (l : InfiniteList α) : l.skip 0 = l := by unfold skip; simp only [Nat.add_zero]
+
+  theorem skip_m_get_sub_eq_get (l : InfiniteList α) (n : Nat) (m : Fin n) : (l.skip m) (n - m) = l n := by 
+    unfold skip
+    simp
+
+  theorem combine_skip_take (l : InfiniteList α) (n : Nat) (m : Fin n) : l.take m ++ (l.skip m).take (n-m) = l.take n := by 
+    induction n with 
+    | zero => 
+      apply False.elim 
+      apply Nat.not_lt_zero
+      apply m.isLt
+    | succ k ih =>
+      have : k.succ - m = (k-m).succ := by 
+        simp only [Nat.succ_eq_add_one]
+        rw [Nat.sub_add_comm]
+        apply Nat.le_of_lt_succ 
+        exact m.isLt
+      rw [this]
+      simp only [take]
+      rw [← Nat.sub_add_comm (by apply Nat.le_of_lt_succ; exact m.isLt)]
+      rw [skip_m_get_sub_eq_get]
+      rw [← List.append_assoc]
+      cases Decidable.em (m < k) with 
+      | inl hl => 
+        rw [ih ⟨m.val, hl⟩]
+      | inr hr => 
+        have : m = k := by cases Nat.lt_or_eq_of_le (Nat.le_of_lt_succ m.isLt); contradiction; assumption
+        rw [this]
+        simp [take]
+end InfiniteList
+
+structure PossiblyInfiniteList (α : Type u) where
+  infinite_list : InfiniteList (Option α)
+  no_holes : ∀ n : Nat, infinite_list n ≠ none -> ∀ m : Fin n, infinite_list m ≠ none
+
+namespace PossiblyInfiniteList
+  def empty : PossiblyInfiniteList α := {
+    infinite_list := fun _ => none
+    no_holes := by intros; contradiction
+  }
+end PossiblyInfiniteList
+
